src/Iris/BI/Extensions.lean
@@ -9,21 +9,21 @@ import Iris.BI.BI
 namespace Iris.BI
 
 /-- Require that a separation logic with the carrier type `PROP` is an affine separation logic. -/
-class BIAffine (PROP : Type) [BI PROP] : Prop where
+class BIAffine (PROP : Type _) [BI PROP] : Prop where
   affine (P : PROP) : Affine P
 
 attribute [instance (default + 100)] BIAffine.affine
 
-class BIPositive (PROP : Type) [BI PROP] where
+class BIPositive (PROP : Type _) [BI PROP] where
   affinely_sep_l {P Q : PROP} : <affine> (P ∗ Q) ⊢ <affine> P ∗ Q
 export BIPositive (affinely_sep_l)
 
-class BILoeb (PROP : Type) [BI PROP] : Prop where
+class BILoeb (PROP : Type _) [BI PROP] : Prop where
   loeb_weak {P : PROP} : (▷ P ⊢ P) → True ⊢ P
 
-class BILaterContractive (PROP : Type) [BI PROP] extends OFE.Contractive later (α := PROP) : Prop
+class BILaterContractive (PROP : Type _) [BI PROP] extends OFE.Contractive later (α := PROP) : Prop
 
-class BIPersistentlyForall (PROP : Type) [BI PROP] where
-  persistently_forall_2 (Ψ : α → PROP) : (∀ a, <pers> (Ψ a)) ⊢ <pers> (∀ a, Ψ a)
+class BIPersistentlyForall (PROP : Type _) [BI PROP] where
+  persistently_sForall_2 (Ψ : PROP → Prop) : (∀ p, ⌜Ψ p⌝ → <pers> p) ⊢ <pers> (sForall Ψ)
 
 end Iris.BI
