src/Iris/ProofMode/Tactics/Clear.lean
@@ -15,7 +15,7 @@ theorem clear_spatial [BI PROP] {P P' A Q : PROP} [TCOr (Affine A) (Absorbing Q)
 theorem clear_intuitionistic [BI PROP] {P P' A Q : PROP}
     (h_rem : P ⊣⊢ P' ∗ □ A) (h : P' ⊢ Q) : P ⊢ Q := clear_spatial h_rem h
 
-def clearCore {prop : Q(Type)} (_bi : Q(BI $prop)) (e e' out goal : Q($prop))
+def clearCore {prop : Q(Type u)} (_bi : Q(BI $prop)) (e e' out goal : Q($prop))
     (pf : Q($e ⊣⊢ $e' ∗ $out)) : MetaM Q(($e' ⊢ $goal) → $e ⊢ $goal) := do
   if out.isAppOfArity ``intuitionistically 3 then
     have out' : Q($prop) := out.appArg!
@@ -29,13 +29,13 @@ elab "iclear" colGt hyp:ident : tactic => do
   let mvar ← getMainGoal
   mvar.withContext do
   let g ← instantiateMVars <| ← mvar.getType
-  let some { prop, bi, e, hyps, goal } := parseIrisGoal? g | throwError "not in proof mode"
+  let some { u, prop, bi, e, hyps, goal } := parseIrisGoal? g | throwError "not in proof mode"
 
   let uniq ← hyps.findWithInfo hyp
   let ⟨e', hyps', out, _, _, _, pf⟩ := hyps.remove true uniq
 
   let m : Q($e' ⊢ $goal) ← mkFreshExprSyntheticOpaqueMVar <|
-    IrisGoal.toExpr { prop, bi, hyps := hyps', goal }
+    IrisGoal.toExpr { u, prop, bi, hyps := hyps', goal }
 
   mvar.assign ((← clearCore bi e e' out goal pf).app m)
   replaceMainGoal [m.mvarId!]
